add skeleton hennessey milner thm

BML/Def.lean
@@ -5,6 +5,7 @@ Authors: see COLLABORATORS.md
 -/
 
 import Mathlib.Data.Set.Basic
+import Mathlib.Data.Set.Finite.Basic
 import Mathlib.Tactic.Tauto
 
 /-!
@@ -35,6 +36,8 @@ structure Model (World : Type) (Atom : Type) where
 inductive Proposition (Atom : Type) : Type where
   /-- Atomic proposition. -/
   | atom (p : Atom)
+  /-- Bottom element. -/
+  | bot
   /-- Negation. -/
   | not (φ : Proposition Atom)
   /-- Conjunction. -/
@@ -53,6 +56,7 @@ variable {φ₁ φ₂ : Proposition Atom}
 /-- M,w ⊨ φ -/
 def eval (M : Model World Atom) (w : World) : Proposition Atom → Prop
   | .atom p => M.v w p
+  | .bot => False
   | .not φ => ¬ eval M w φ
   | .and φ₁ φ₂ => eval M w φ₁ ∧ eval M w φ₂
   | .diamond φ => ∃ x : World, M.r w x ∧ eval M x φ
@@ -110,7 +114,7 @@ class Bisimulation {World1 World2 : Type} {Atom : Type}
   Z : World1 → World2 → Prop
 
   /- Z is non-empty -/
-  nonempty : ∃ w1 w2, Z w1 w2
+  -- nonempty : ∃ w1 w2, Z w1 w2
 
   /- Related world have the same proposition letters -/
   same_atoms : ∀ w1 w2, Z w1 w2 → ∀ p, M1.v w1 p ↔ M2.v w2 p
@@ -131,6 +135,8 @@ theorem bisimular_worlds_are_modally_equivalent {World1 World2 : Type} {Atom : T
   induction φ generalizing w1 w2 h with
   | atom p =>
     exact B.same_atoms w1 w2 h p
+  | bot =>
+    simp only [Proposition.eval]
   | not ψ ih =>
     simp only [Proposition.eval]
     rw [ih]
@@ -155,5 +161,105 @@ theorem bisimular_worlds_are_modally_equivalent {World1 World2 : Type} {Atom : T
       constructor
       · exact hr'
       · exact (ih v1 v2 hZ).mpr hψ
+
+
+/- Image-finite definition for model with 1 relation-/
+def image_finite {World Atom : Type} (M : Model World Atom) : Prop :=
+  ∀ w, Set.Finite {v | M.r w v}
+
+
+/-- Theorem 2.20: Hennessey-Milner -/
+theorem hennessey_milner
+  {World1 World2 Atom : Type}
+  {M1 : Model World1 Atom}
+  {M2 : Model World2 Atom}
+  (h1 : image_finite M1)
+  (h2 : image_finite M2)
+  (w1 : World1) (w2 : World2) :
+  (∃ B : Bisimulation M1 M2, B.Z w1 w2) ↔
+  (∀ φ, Proposition.eval M1 w1 φ ↔ Proposition.eval M2 w2 φ) := by
+  constructor
+  /- This is theorem 2.20 -/
+  · intro h
+    obtain ⟨B, hZ⟩ := h
+    exact bisimular_worlds_are_modally_equivalent B w1 w2 hZ
+  /- Prove that modal equivalence is a bisimulation -/
+  · intro h
+    let Z : World1 → World2 → Prop := fun w1 w2 => ∀ φ, Proposition.eval M1 w1 φ ↔ Proposition.eval M2 w2 φ
+    /- Same atoms -/
+    have same_atoms : ∀ w1 w2, Z w1 w2 → ∀ p, (M1.v w1 p ↔ M2.v w2 p) := by
+      intro w1 w2 hZ
+      intro p
+      specialize hZ (Proposition.atom p)
+      exact hZ
+    /- Forth condition -/
+    have forth : ∀ w1 w2 v1, Z w1 w2 → M1.r w1 v1 → ∃ v2, M2.r w2 v2 ∧ Z v1 v2 := by
+      intro w1 w2 v1 hZ hr
+      classical
+      by_contra
+      /- Define S' -/
+      let S' : Set World2 := {v2 | M2.r w2 v2}
+      /- Show that S' is non-empty -/
+      have hS' : ∃ v2, M2.r w2 v2 := by
+        by_contra hhS'
+        /- M2, w2 ⊩ □ ⊥ -/
+        have boxBot : Proposition.eval M2 w2 (Proposition.bot.box) := by
+          unfold Proposition.box
+          simp only [Proposition.eval, not_exists, not_and, not_not]
+          intro v2 hr
+          exact hhS' ⟨v2, hr⟩
+        /- M1, w1 ⊩ ◇ ⊤ -/
+        have diamondTop : Proposition.eval M1 w1 (Proposition.bot.not.diamond) := by
+          use v1
+          constructor
+          · exact hr
+          · exact False.elim
+        /- M2, w2 ⊩ ◇ ⊤ -/
+        have diamondTop' : Proposition.eval M2 w2 (Proposition.bot.not.diamond) := by
+          specialize hZ (Proposition.bot.not.diamond)
+          exact hZ.mp diamondTop
+        /- Now derive the contradiction -/
+        unfold Proposition.eval at diamondTop'
+        simp only [Proposition.eval] at diamondTop'
+        rw [Proposition.eval_box] at boxBot
+        unfold Proposition.eval at boxBot
+        rcases diamondTop' with ⟨v2, hr', h⟩
+        specialize boxBot v2 hr'
+        exact boxBot
+      /- Show that S' is finite by image-finiteness -/
+      have hS'finite : Set.Finite S' := by
+        apply h2 w2
+      /- Now, build the formula using S' -/
+      /- First prove that for each w' ∈ S', the ψ in the book exists -/
+      have phi_exists_for_each_member_of_Sp :
+        ∀ w' ∈ S', ∃ ψ , Proposition.eval M1 v1 ψ ∧ ¬ Proposition.eval M2 w' ψ := by
+        intro w' hw'
+        /- w' is neighbor of w2 -/
+        have hr' : M2.r w2 w' := hw'
+        push Not at this
+        specialize this w' hr'
+        unfold Z at this
+        push Not at this
+        rcases this with ⟨ψ, hψ⟩
+        rcases hψ with ⟨hψ1, hψ2⟩
+        use ψ
+        use ψ.not
+        simp only [Proposition.eval, not_not]
+        tauto
+      /- Now, construct the finite conjunction of these formulas -/
+      sorry
+    /- Back condition -/
+    have back : ∀ w1 w2 v2, Z w1 w2 → M2.r w2 v2 → ∃ v1, M1.r w1 v1 ∧ Z v1 v2 := by
+      sorry
+
+    /- Construct the bisimulation -/
+    use { Z := Z, same_atoms := same_atoms, forth := forth, back := back }
+
+
+
+
+
+
+
 
 end BML
